pcuic/theories/PCUICReduction.v
@@ -133,8 +133,8 @@ Inductive red1 (Σ : global_env) (Γ : context) : term -> term -> Type :=
 (** Case *)
 | red_iota ci c u args p brs br :
     nth_error brs c = Some br ->
-    (* #|p.(pparams)| = ci.(ind_npars) ->
-    #|skipn (ci_npar ci) args| = context_assumptions br.(bcontext) -> *)
+    (* #|p.(pparams)| = ci.(ind_npars) ->*)
+    #|skipn (ci_npar ci) args| = context_assumptions br.(bcontext) ->
     red1 Σ Γ (tCase ci p (mkApps (tConstruct ci.(ci_ind) c u) args) brs)
          (iota_red ci.(ci_npar) args br)
 
@@ -235,6 +235,7 @@ Lemma red1_ind_all :
        (forall (Γ : context) (ci : case_info) (c : nat) (u : Instance.t) (args : list term)
           (p : predicate term) (brs : list (branch term)) br,
           nth_error brs c = Some br ->
+          #|skipn (ci_npar ci) args| = context_assumptions br.(bcontext) ->
           P Γ (tCase ci p (mkApps (tConstruct ci.(ci_ind) c u) args) brs)
               (iota_red ci.(ci_npar) args br)) ->
 
